Remove another unneeded arg. from crash_inv predicates.

src/program_logic/crash_inv.v
@@ -19,25 +19,25 @@ Implicit Types Φc : iProp Σ.
 Implicit Types v : val Λ.
 Implicit Types e : expr Λ.
 
-Definition crash_inv N k E P :=
-  (∃ γ γ', staged_inv N k (E ∖ ↑N) (E ∖ ↑N) γ γ' P)%I.
+Definition crash_inv N k P :=
+  (∃ γ γ', staged_inv N k (⊤ ∖ ↑N) (⊤ ∖ ↑N) γ γ' P)%I.
 
-Definition crash_inv_full N k E Q P :=
-  (∃ γ γ' Qr, staged_inv N k (E ∖ ↑N) (E ∖ ↑N) γ γ' P ∗ staged_value N γ Q Qr ∗ □ (Q -∗ P))%I.
+Definition crash_inv_full N k Q P :=
+  (∃ γ γ' Qr, staged_inv N k (⊤ ∖ ↑N) (⊤ ∖ ↑N) γ γ' P ∗ staged_value N γ Q Qr ∗ □ (Q -∗ P))%I.
 
-Definition crash_inv_pending N k E P :=
-  (∃ γ γ', staged_inv N k (E ∖ ↑N) (E ∖ ↑N) γ γ' P ∗ staged_pending γ')%I.
+Definition crash_inv_pending N k P :=
+  (∃ γ γ', staged_inv N k (⊤ ∖ ↑N) (⊤ ∖ ↑N) γ γ' P ∗ staged_pending γ')%I.
 
-Global Instance crash_inv_pers N k E P : Persistent (crash_inv N k E P).
+Global Instance crash_inv_pers N k P : Persistent (crash_inv N k P).
 Proof. apply _. Qed.
 
-Lemma crash_inv_alloc N k E E' P Q:
+Lemma crash_inv_alloc N k E P Q:
   ▷ Q ∗ □ (Q -∗ P) ={E}=∗
-  crash_inv_full N k E' Q P ∗ crash_inv_pending N k E' P.
+  crash_inv_full N k Q P ∗ crash_inv_pending N k P.
 Proof.
   iIntros "HQP".
   iDestruct "HQP" as "(HQ&#HQP)".
-  iMod (staged_inv_alloc N k E (E' ∖ ↑N) P Q True%I with "[HQ]") as (γ γ') "(#Hinv&Hval&Hpend)".
+  iMod (staged_inv_alloc N k E (⊤ ∖ ↑N) P Q True%I with "[HQ]") as (γ γ') "(#Hinv&Hval&Hpend)".
   { iFrame. iAlways. iIntros. iDestruct ("HQP" with "[$]") as "$". }
   iModIntro.
   iSplitL "Hval".
@@ -45,30 +45,29 @@ Proof.
   - iExists γ, _. iFrame. iFrame "Hinv".
 Qed.
 
-Lemma crash_inv_full_impl N k E Q P:
-  crash_inv_full N k E Q P -∗ □ (Q -∗ P).
+Lemma crash_inv_full_impl N k Q P:
+  crash_inv_full N k Q P -∗ □ (Q -∗ P).
 Proof. iIntros "H". iDestruct "H" as (???) "(?&?&$)"; eauto. Qed.
 
-Lemma crash_inv_full_weaken N k E Q P:
-  crash_inv_full N k E Q P -∗ crash_inv N k E P.
+Lemma crash_inv_full_weaken N k Q P:
+  crash_inv_full N k Q P -∗ crash_inv N k P.
 Proof. iIntros "H". iDestruct "H" as (???) "(?&?)"; eauto. iExists _, _. iFrame. Qed.
 
-Lemma crash_inv_pending_weaken N k E P:
-  crash_inv_pending N k E P -∗ crash_inv N k E P.
+Lemma crash_inv_pending_weaken N k P:
+  crash_inv_pending N k P -∗ crash_inv N k P.
 Proof. iIntros "H". iDestruct "H" as (??) "(?&?)"; eauto. iExists _, _. iFrame. Qed.
 
-Lemma wpc_crash_inv_open s k k' E1 E1' E2 e Φ Φc Q P N:
-  E1 ⊆ E1' →
+Lemma wpc_crash_inv_open s k k' E1 E2 e Φ Φc Q P N:
   ↑N ⊆ E1 →
   S k < k' →
   to_val e = None →
-  crash_inv_full N (LVL k') E1' Q P -∗
+  crash_inv_full N (LVL k') Q P -∗
   (Φc ∧ (Q -∗ WPC e @ NotStuck; (LVL k); (E1 ∖ ↑N); ∅
-                    {{λ v, Q ∗ (crash_inv_full N (LVL k') E1' Q P -∗ (Φ v ∧ Φc))}}
+                    {{λ v, Q ∗ (crash_inv_full N (LVL k') Q P -∗ (Φ v ∧ Φc))}}
                     {{ Φc ∗ P }})) -∗
   WPC e @ s; LVL (S (S k)); E1; E2 {{ Φ }} {{ Φc }}.
 Proof.
-  iIntros (????) "Hfull Hwp".
+  iIntros (???) "Hfull Hwp".
   iDestruct "Hfull" as (???) "(#Hinv&Hval&#Hwand)".
   iApply (wpc_staged_inv_open _ _ _ _ _ _ _ _ _ _ _ (λ _, Q)); eauto.
   iFrame "Hinv". iFrame.
@@ -85,18 +84,17 @@ Proof.
   - iIntros. rewrite difference_diag_L. iModIntro; eauto.
 Qed.
 
-Lemma wpc_crash_inv_open_modify Qnew s k k' E1 E1' E2 e Φ Φc Q P N :
-  E1 ⊆ E1' →
+Lemma wpc_crash_inv_open_modify Qnew s k k' E1 E2 e Φ Φc Q P N :
   ↑N ⊆ E1 →
   S k < k' →
   to_val e = None →
-  crash_inv_full N (LVL k') E1' Q P -∗
+  crash_inv_full N (LVL k') Q P -∗
   (Φc ∧ (Q -∗ WPC e @ NotStuck; (LVL k); (E1 ∖ ↑N); ∅
-                    {{λ v, Qnew v ∗ □ (Qnew v -∗ P)  ∗ (crash_inv_full N (LVL k') E1' (Qnew v) P -∗ (Φ v ∧ Φc))}}
+                    {{λ v, Qnew v ∗ □ (Qnew v -∗ P)  ∗ (crash_inv_full N (LVL k') (Qnew v) P -∗ (Φ v ∧ Φc))}}
                     {{ Φc ∗ P }})) -∗
   WPC e @ s; LVL (S (S k)); E1; E2 {{ Φ }} {{ Φc }}.
 Proof.
-  iIntros (????) "Hfull Hwp".
+  iIntros (???) "Hfull Hwp".
   iDestruct "Hfull" as (???) "(#Hinv&Hval&#Hwand)".
   iApply (wpc_staged_inv_open _ _ _ _ _ _ _ _ _ _ _ Qnew); eauto.
   iFrame "Hinv". iFrame.
@@ -112,22 +110,21 @@ Proof.
   - iIntros. rewrite difference_diag_L. iModIntro; eauto.
 Qed.
 
-Lemma wpc_crash_inv_init s k k' N E1 E2 e Φ Φc P :
+Lemma wpc_crash_inv_init s k k' N E2 e Φ Φc P :
   k' < k →
-  ↑N ⊆ E1 →
-  crash_inv_pending N (LVL k') E1 P ∗
-  WPC e @ s; LVL k; E1; E2 {{ Φ }} {{ Φc }} ⊢
-  WPC e @ s; LVL (S k); E1; E2 {{ Φ }} {{ Φc ∗ P }}.
+  crash_inv_pending N (LVL k') P ∗
+  WPC e @ s; LVL k; ⊤; E2 {{ Φ }} {{ Φc }} ⊢
+  WPC e @ s; LVL (S k); ⊤; E2 {{ Φ }} {{ Φc ∗ P }}.
 Proof.
-  iIntros (??) "(H&?)".
+  iIntros (?) "(H&?)".
   iDestruct "H" as (??) "(?&?)".
   iApply wpc_staged_inv_init; last (by iFrame); eauto.
 Qed.
 
-Lemma crash_inv_open_modify N k' k E E' E1 P Q R:
+Lemma crash_inv_open_modify N k' k E E' P Q R:
   ↑N ⊆ E →
-  crash_inv_full N k' E1 Q P -∗
-  ((Q ∗ (∀ Q', ▷ Q' ∗ □ (Q' -∗ P) ={E∖↑N,E}=∗ crash_inv_full N k' E1 Q' P)) ∨ (C ∗ |={E∖↑N, E}=> crash_inv_full N k' E1 Q P)
+  crash_inv_full N k' Q P -∗
+  ((Q ∗ (∀ Q', ▷ Q' ∗ □ (Q' -∗ P) ={E∖↑N,E}=∗ crash_inv_full N k' Q' P)) ∨ (C ∗ |={E∖↑N, E}=> crash_inv_full N k' Q P)
    -∗ |={E ∖ ↑N, E'}_k=> R) -∗
   (|={E,E'}_(S (S k))=> R).
 Proof.
@@ -149,10 +146,10 @@ Proof.
   - iRight. iFrame. iMod "Hclo". iModIntro. iExists _, _, _. iFrame "Hclo Hwand Hinv".
 Qed.
 
-Lemma crash_inv_open N k' k E E' E1 P Q R:
+Lemma crash_inv_open N k' k E E' P Q R:
   ↑N ⊆ E →
-  crash_inv_full N k' E1 Q P -∗
-  ((Q ∗ (▷ Q ={E∖↑N,E}=∗ crash_inv_full N k' E1 Q P)) ∨ (C ∗ |={E∖↑N, E}=> crash_inv_full N k' E1 Q P)
+  crash_inv_full N k' Q P -∗
+  ((Q ∗ (▷ Q ={E∖↑N,E}=∗ crash_inv_full N k' Q P)) ∨ (C ∗ |={E∖↑N, E}=> crash_inv_full N k' Q P)
    -∗ |={E ∖ ↑N, E'}_k=> R) -∗
   (|={E,E'}_(S (S k))=> R).
 Proof.
